Added for counter pattern and associated Hoare logic laws

UTP/ITree_Hoare.thy
@@ -172,11 +172,24 @@ next
     by (simp add: for_Cons del: SEXP_apply, meson "1" "2" hl_seq)
 qed
 
+text \<open> For loops with invariant annotations \<close>
+
 definition for_inv :: "'i list \<Rightarrow> (nat \<Rightarrow> (bool, 's) expr) \<Rightarrow> ('i \<Rightarrow> ('e, 's) htree) \<Rightarrow> ('e, 's) htree" where
 "for_inv I P S = for_itree I S"
 
-syntax "_for_inv_itree" :: "id \<Rightarrow> logic \<Rightarrow> id \<Rightarrow> logic \<Rightarrow> logic \<Rightarrow> logic" ("for _ in _ inv _. _ do _ od")
-translations "_for_inv_itree x I i P S" == "CONST for_inv I (\<lambda> i. (P)\<^sub>e) (\<lambda> x. S)"
+text \<open> For loops counting for m to n with invariant annotations. We use a new constant, as the form
+  of invariant can be simplified in this case. \<close>
+
+definition for_to_inv :: "nat \<Rightarrow> nat \<Rightarrow> (nat \<Rightarrow> (bool, 's) expr \<times> ('e, 's) htree) \<Rightarrow> ('e, 's) htree" where
+"for_to_inv m n IC \<equiv> for_inv [m..<n+1] (\<lambda> i. fst (IC (i + m))) (\<lambda> i. snd (IC i))"
+
+syntax 
+  "_for_inv_itree" :: "id \<Rightarrow> logic \<Rightarrow> id \<Rightarrow> logic \<Rightarrow> logic \<Rightarrow> logic" ("for _ in _ inv _. _ do _ od")
+  "_for_to_inv_itree"   :: "id \<Rightarrow> logic \<Rightarrow> logic \<Rightarrow> logic \<Rightarrow> logic \<Rightarrow> logic \<Rightarrow> logic" ("for _ := _ to _ inv _ do _ od")
+
+translations 
+  "_for_inv_itree x I i P S" == "CONST for_inv I (\<lambda> i. (P)\<^sub>e) (\<lambda> x. S)"
+  "for i := m to n inv I do C od" == "CONST for_to_inv m n (\<lambda> i. ((I)\<^sub>e, C))"
 
 lemma hoare_for_inv [hoare_safe]:
   assumes "\<And> i. i < length xs \<Longrightarrow> \<^bold>{@(R i)\<^bold>} S (xs ! i) \<^bold>{@(R (i+1))\<^bold>}"
@@ -184,6 +197,17 @@ lemma hoare_for_inv [hoare_safe]:
   shows "\<^bold>{P\<^bold>} for x in xs inv i. @(R i) do S x od \<^bold>{Q\<^bold>}"
   unfolding for_inv_def
   by (meson assms hl_conseq hl_for)
+
+lemma hl_for_to_inv [hoare_safe]:
+  assumes "\<And>i. \<lbrakk> m \<le> i; i \<le> n \<rbrakk> \<Longrightarrow> \<^bold>{@(R i)\<^bold>} S i \<^bold>{@(R (i + 1))\<^bold>}"
+   "`P \<longrightarrow> @(R m)`" "`@(R (n+1 - m+m)) \<longrightarrow> Q`"
+  shows "\<^bold>{P\<^bold>} for i := m to n inv @(R i) do S i od \<^bold>{Q\<^bold>}"
+  unfolding for_to_inv_def fst_conv snd_conv
+  using assms
+  apply (rule_tac hoare_for_inv, simp_all only: length_upt)
+  apply (metis ab_semigroup_add_class.add_ac(1) add.commute assms(1) le_add2 less_Suc_eq_le less_diff_conv nth_upt plus_1_eq_Suc)
+  apply (simp add: assms(2))
+  done 
 
 lemma hoare_while_partial [hoare_safe]:
   assumes "\<^bold>{P \<and> B\<^bold>} S \<^bold>{P\<^bold>}"
